fix definitions

src/DiceCore.fst
@@ -2,45 +2,33 @@ module DiceCore
 
 open LowStar.BufferOps
 open LowStar.Modifies
-open FStar.HyperStack.ST
-  
+open LowStar.Buffer
+open FStar.Integers
+
 module HS  = FStar.HyperStack
 module HST = FStar.HyperStack.ST
-module B   = FStar.Buffer
+module B   = LowStar.Buffer
+module IB  = LowStar.ImmutableBuffer
 module M   = LowStar.Modifies
-module U64 = FStar.UInt64
-module U32 = FStar.UInt32
-module U16 = FStar.UInt16
-module U8  = FStar.UInt8
-module Bytes = FStar.Bytes
 
-let uint64 = U64.t
-let uint32 = U32.t
-let uint16 = U16.t
-let uint8  = U8.t
-let bytes   = Bytes.bytes
+let _DICE_UDS_LENGTH    : uint_32 = 0x20ul
+let _DICE_DIGEST_LENGTH : uint_32 = 0x20ul
 
-let _DICE_UDS_LENGTH    : U32.t = 0x20ul
-let _DICE_DIGEST_LENGTH : U32.t = 0x20ul
-
-let f () : St unit =
+let f () : HST.St unit =
   let l = LowStar.Buffer.malloc HS.root 0uy 8ul in
   LowStar.Buffer.free l
 
-/// FStar.Buffer or LowStar.Buffer?
+let x = LowStar.Buffer.malloc HS.root 0uy 8ul
 
-let test () : St unit =
-  let h = B.create 0 8ul in
-
-
-  let udslist = [
+inline_for_extraction let udsContent = [
     0xb5; 0x85; 0x94; 0x93; 0x66; 0x1e; 0x2e; 0xae;
     0x96; 0x77; 0xc5; 0x5d; 0x59; 0x0b; 0x92; 0x94;
     0xe0; 0x94; 0xab; 0xaf; 0xd7; 0x40; 0x78; 0x7e;
     0x05; 0x0d; 0xfe; 0x6d; 0x85; 0x90; 0x53; 0xa0
-    ] in
-  let _UDS = B.malloc HS.root udslist 1ul in
-  let y = B.alloca_of_list udslist in
+    ]
+
+let test () : HST.St unit =
+  let _UDS = IB.igcmalloc_of_list HS.root udsContent in
   ()
 
 let _CDI = B.malloc HS.root [0x00] _DICE_DIGEST_LENGTH
@@ -61,38 +49,31 @@ let _RIOT_ENTRY : string = "RiotStart"
 // NOTE: Getting familiar with F* and DICE/RIoT by simply re-implement reference code (https://github.com/microsoft/RIoT/blob/master/Reference/RIoT/Core/RIoT.cpp) in F*.
 
 (*digest lengths*)
-assume val _SHA256_DIGEST_LENGTH : U32.t
-assume val _RIOT_DIGEST_LENGTH : uint32
+assume val _SHA256_DIGEST_LENGTH : uint_32
+assume val _RIOT_DIGEST_LENGTH : uint_32
 
-assume val _RIOT_LABEL_IDENTITY : uint32
-assume val _RIOT_LABEL_IDENTITY_SIZE : uint32
-(*
-let on_the_heap ():St UInt64.t =
+assume val _RIOT_LABEL_IDENTITY : uint_32
+assume val _RIOT_LABEL_IDENTITY_SIZE : uint_32
+
+let on_the_heap () : HST.St UInt64.t =
 let b = B.malloc HS.root 0uL 64ul in
   b.(0ul) <- 32uL;
   let r = b.(0ul) in
   B.free b;
   r
 
-assume val _fwImage : uint32
-assume val _fwSize : uint32
-
-effect ST
-  (a:Type)
-  (pre :HS.mem -> Type0)
-  (post:HS.mem -> a -> HS.mem -> Type0)
-= FStar.HyperStack.ST.ST a pre post
-
-effect St (a:Type) = FStar.HyperStack.ST.St a
+assume val _fwImage : uint_32
+assume val _fwSize : uint_32
 
 val _DICEStart
   (riotImagePath   : string)
   (loaderImagePath : string)
-: ST unit
+: HST.ST unit
   (requires fun h -> True)
   (ensures  fun h0 _ h1 -> True)
-let _DICEStart _ =
+let _DICEStart _ _ =
   let uDigest = B.malloc HS.root 0ul _DICE_DIGEST_LENGTH in
   let rDigest = B.malloc HS.root 0ul _DICE_DIGEST_LENGTH in
+  let _UDS = IB.igcmalloc_of_list HS.root udsContent in
   ()
- 
+
